Data/Fin0.hs
@@ -4,8 +4,9 @@ import qualified Prelude
 import qualified Data.List
 import qualified Data.Compare as Compare
 import qualified Data.Compare_dec as Compare_dec
+import qualified Data.Datatypes as Datatypes
 import qualified Data.Fin as Fin
-import qualified Data.Peano as Peano
+import qualified Data.Logic as Logic
 
 
 type Coq_fin = Fin.Coq_t
@@ -18,19 +19,11 @@ fin_to_nat :: Prelude.Int -> Coq_fin -> Prelude.Int
 fin_to_nat n f =
    (Fin.to_nat n f)
 
-ultimate_from_nat :: Prelude.Int -> Coq_fin
-ultimate_from_nat n =
-  from_nat n (Peano.pred n)
-
-pred_fin :: Prelude.Int -> Coq_fin -> Prelude.Maybe Coq_fin
-pred_fin n f =
-  let {f0 = Fin.to_nat n f} in
-  (\fO fS n -> if n Prelude.== 0 then fO () else fS (n Prelude.- 1))
-    (\_ ->
-    Prelude.Nothing)
-    (\x -> Prelude.Just
-    (from_nat n x))
-    f0
+fin_Sn_inv :: Prelude.Int -> a1 -> (Coq_fin -> a1) -> Coq_fin -> a1
+fin_Sn_inv n pO pS x =
+  case x of {
+   Fin.F1 n0 -> pO;
+   Fin.FS n0 y -> pS y}
 
 fin_compare :: Prelude.Int -> Coq_fin -> Coq_fin -> Prelude.Ordering
 fin_compare n x y =
@@ -39,4 +32,13 @@ fin_compare n x y =
 fin_CompareSpec :: Prelude.Int -> Compare.CompareSpec Coq_fin
 fin_CompareSpec n =
   fin_compare n
+
+fin_expand :: Prelude.Int -> Fin.Coq_t -> Fin.Coq_t
+fin_expand n p =
+  Datatypes.nat_rec (\p0 ->
+    case p0 of {
+     Fin.F1 n0 -> Logic.coq_False_rec;
+     Fin.FS n0 h -> Logic.coq_False_rec h}) (\n0 iHn p0 ->
+    fin_Sn_inv n0 (Fin.F1 (Prelude.succ n0)) (\y -> Fin.FS (Prelude.succ n0)
+      (iHn y)) p0) n p
 
