Data/Main.hs
@@ -1,9 +1,13 @@
+{-# OPTIONS_GHC -cpp -fglasgow-exts #-}
+{- For Hugs, use the option -F"cpp -P -traditional" -}
+
 module Data.Main where
 
 import qualified Prelude
 import qualified Data.List
 import qualified Data.Compare as Compare
 import qualified Data.Compare_dec as Compare_dec
+import qualified Data.Datatypes as Datatypes
 import qualified Data.EqNat as EqNat
 import qualified Data.Fin0 as Fin0
 import qualified Data.Fin as Fin
@@ -12,8 +16,23 @@ import qualified Data.Lib as Lib
 import qualified Data.List0 as List0
 import qualified Data.Logic as Logic
 import qualified Data.NPeano as NPeano
+import qualified Data.Peano as Peano
+import qualified Data.Plus as Plus
 import qualified Data.Specif as Specif
+import qualified Data.Vector1 as Vector1
+import qualified Data.Vector0 as Vector0
 
+
+
+--unsafeCoerce :: a -> b
+#ifdef __GLASGOW_HASKELL__
+import qualified GHC.Base as GHC.Base
+unsafeCoerce = GHC.Base.unsafeCoerce#
+#else
+-- HUGS
+import qualified Data.IOExts as IOExts
+unsafeCoerce = IOExts.unsafeCoerce
+#endif
 
 __ :: any
 __ = Prelude.error "Logical or arity value used"
@@ -34,22 +53,336 @@ _LinearScan__maxReg =
 
 type LinearScan__PhysReg = Fin0.Coq_fin
 
+data LinearScan__V__Coq_t a =
+   LinearScan__V__Coq_nil
+ | LinearScan__V__Coq_cons a Prelude.Int (LinearScan__V__Coq_t a)
+
+_LinearScan__V__t_rect :: a2 -> (a1 -> Prelude.Int -> (LinearScan__V__Coq_t
+                          a1) -> a2 -> a2) -> Prelude.Int ->
+                          (LinearScan__V__Coq_t a1) -> a2
+_LinearScan__V__t_rect f f0 n t =
+  case t of {
+   LinearScan__V__Coq_nil -> f;
+   LinearScan__V__Coq_cons h n0 t0 ->
+    f0 h n0 t0 (_LinearScan__V__t_rect f f0 n0 t0)}
+
+_LinearScan__V__t_rec :: a2 -> (a1 -> Prelude.Int -> (LinearScan__V__Coq_t
+                         a1) -> a2 -> a2) -> Prelude.Int ->
+                         (LinearScan__V__Coq_t a1) -> a2
+_LinearScan__V__t_rec =
+  _LinearScan__V__t_rect
+
+_LinearScan__V__rectS :: (a1 -> a2) -> (a1 -> Prelude.Int ->
+                         (LinearScan__V__Coq_t a1) -> a2 -> a2) ->
+                         Prelude.Int -> (LinearScan__V__Coq_t a1) -> a2
+_LinearScan__V__rectS bas rect n v =
+  case v of {
+   LinearScan__V__Coq_nil -> unsafeCoerce (\_ -> Logic.coq_False_rect);
+   LinearScan__V__Coq_cons a n0 v0 ->
+    (\fO fS n -> if n Prelude.== 0 then fO () else fS (n Prelude.- 1))
+      (\_ ->
+      case v0 of {
+       LinearScan__V__Coq_nil -> bas a;
+       LinearScan__V__Coq_cons h n1 t ->
+        unsafeCoerce (\_ -> Logic.coq_False_rect)})
+      (\nn' ->
+      rect a nn' v0 (_LinearScan__V__rectS bas rect nn' v0))
+      n0}
+
+_LinearScan__V__rect2 :: a3 -> (Prelude.Int -> (LinearScan__V__Coq_t 
+                         a1) -> (LinearScan__V__Coq_t a2) -> a3 -> a1 -> a2
+                         -> a3) -> Prelude.Int -> (LinearScan__V__Coq_t 
+                         a1) -> (LinearScan__V__Coq_t a2) -> a3
+_LinearScan__V__rect2 bas rect n v1 v2 =
+  case v1 of {
+   LinearScan__V__Coq_nil ->
+    case v2 of {
+     LinearScan__V__Coq_nil -> bas;
+     LinearScan__V__Coq_cons h n0 t ->
+      unsafeCoerce (\_ -> Logic.coq_False_rect)};
+   LinearScan__V__Coq_cons h1 n0 t1 ->
+    case v2 of {
+     LinearScan__V__Coq_nil -> Logic.coq_False_rect;
+     LinearScan__V__Coq_cons h2 n1 t2 ->
+      rect n1 t1 t2 (_LinearScan__V__rect2 bas rect n1 t1 t2) h1 h2}}
+
+_LinearScan__V__case0 :: a2 -> (LinearScan__V__Coq_t a1) -> a2
+_LinearScan__V__case0 h v =
+  case v of {
+   LinearScan__V__Coq_nil -> h;
+   LinearScan__V__Coq_cons h0 n t -> unsafeCoerce (\_ -> Datatypes.id)}
+
+_LinearScan__V__caseS :: (a1 -> Prelude.Int -> (LinearScan__V__Coq_t 
+                         a1) -> a2) -> Prelude.Int -> (LinearScan__V__Coq_t
+                         a1) -> a2
+_LinearScan__V__caseS h n v =
+  case v of {
+   LinearScan__V__Coq_nil -> __;
+   LinearScan__V__Coq_cons h0 n0 t -> h h0 n0 t}
+
+_LinearScan__V__hd :: Prelude.Int -> (LinearScan__V__Coq_t a1) -> a1
+_LinearScan__V__hd n v =
+  case v of {
+   LinearScan__V__Coq_nil -> __;
+   LinearScan__V__Coq_cons h n0 t -> h}
+
+_LinearScan__V__last :: Prelude.Int -> (LinearScan__V__Coq_t a1) -> a1
+_LinearScan__V__last n v =
+  let {bas = \a -> a} in
+  let {rect = \a n0 v0 h -> h} in
+  let {
+   rectS_fix n0 v0 =
+     case v0 of {
+      LinearScan__V__Coq_nil ->
+       unsafeCoerce (\_ -> Prelude.error "absurd case");
+      LinearScan__V__Coq_cons a n1 v1 ->
+       (\fO fS n -> if n Prelude.== 0 then fO () else fS (n Prelude.- 1))
+         (\_ ->
+         case v1 of {
+          LinearScan__V__Coq_nil -> bas a;
+          LinearScan__V__Coq_cons h n2 t ->
+           unsafeCoerce (\_ -> Prelude.error "absurd case")})
+         (\nn' ->
+         rect a nn' v1 (rectS_fix nn' v1))
+         n1}}
+  in rectS_fix n v
+
+_LinearScan__V__const :: a1 -> Prelude.Int -> LinearScan__V__Coq_t a1
+_LinearScan__V__const a n =
+  (\fO fS n -> if n Prelude.== 0 then fO () else fS (n Prelude.- 1))
+    (\_ ->
+    LinearScan__V__Coq_nil)
+    (\n0 -> LinearScan__V__Coq_cons a n0
+    (_LinearScan__V__const a n0))
+    n
+
+_LinearScan__V__nth :: Prelude.Int -> (LinearScan__V__Coq_t a1) -> Fin.Coq_t
+                       -> a1
+_LinearScan__V__nth m v' p =
+  case p of {
+   Fin.F1 q -> _LinearScan__V__caseS (\h n t -> h) q v';
+   Fin.FS q p' ->
+    _LinearScan__V__caseS (\h n t p0 -> _LinearScan__V__nth n t p0) q v' p'}
+
+_LinearScan__V__nth_order :: Prelude.Int -> (LinearScan__V__Coq_t a1) ->
+                             Prelude.Int -> a1
+_LinearScan__V__nth_order n v p =
+  _LinearScan__V__nth n v (Fin.of_nat_lt p n)
+
+_LinearScan__V__replace :: Prelude.Int -> (LinearScan__V__Coq_t a1) ->
+                           Fin.Coq_t -> a1 -> LinearScan__V__Coq_t a1
+_LinearScan__V__replace n v p a =
+  case p of {
+   Fin.F1 k ->
+    _LinearScan__V__caseS (\h n0 t -> LinearScan__V__Coq_cons a n0 t) k v;
+   Fin.FS k p' ->
+    _LinearScan__V__caseS (\h n0 t p2 -> LinearScan__V__Coq_cons h n0
+      (_LinearScan__V__replace n0 t p2 a)) k v p'}
+
+_LinearScan__V__replace_order :: Prelude.Int -> (LinearScan__V__Coq_t 
+                                 a1) -> Prelude.Int -> a1 ->
+                                 LinearScan__V__Coq_t a1
+_LinearScan__V__replace_order n v p =
+  _LinearScan__V__replace n v (Fin.of_nat_lt p n)
+
+_LinearScan__V__tl :: Prelude.Int -> (LinearScan__V__Coq_t a1) ->
+                      LinearScan__V__Coq_t a1
+_LinearScan__V__tl n v =
+  case v of {
+   LinearScan__V__Coq_nil -> __;
+   LinearScan__V__Coq_cons h n0 t -> t}
+
+_LinearScan__V__shiftout :: Prelude.Int -> (LinearScan__V__Coq_t a1) ->
+                            LinearScan__V__Coq_t a1
+_LinearScan__V__shiftout n v =
+  case v of {
+   LinearScan__V__Coq_nil -> unsafeCoerce (\_ -> Prelude.error "absurd case");
+   LinearScan__V__Coq_cons a n0 v0 ->
+    (\fO fS n -> if n Prelude.== 0 then fO () else fS (n Prelude.- 1))
+      (\_ ->
+      case v0 of {
+       LinearScan__V__Coq_nil -> LinearScan__V__Coq_nil;
+       LinearScan__V__Coq_cons h n1 t ->
+        unsafeCoerce (\_ -> Prelude.error "absurd case")})
+      (\nn' -> LinearScan__V__Coq_cons a nn'
+      (_LinearScan__V__shiftout nn' v0))
+      n0}
+
+_LinearScan__V__shiftin :: Prelude.Int -> a1 -> (LinearScan__V__Coq_t 
+                           a1) -> LinearScan__V__Coq_t a1
+_LinearScan__V__shiftin n a v =
+  case v of {
+   LinearScan__V__Coq_nil -> LinearScan__V__Coq_cons a 0
+    LinearScan__V__Coq_nil;
+   LinearScan__V__Coq_cons h n0 t -> LinearScan__V__Coq_cons h (Prelude.succ
+    n0) (_LinearScan__V__shiftin n0 a t)}
+
+_LinearScan__V__shiftrepeat :: Prelude.Int -> (LinearScan__V__Coq_t a1) ->
+                               LinearScan__V__Coq_t a1
+_LinearScan__V__shiftrepeat n v =
+  case v of {
+   LinearScan__V__Coq_nil -> unsafeCoerce (\_ -> Prelude.error "absurd case");
+   LinearScan__V__Coq_cons a n0 v0 ->
+    (\fO fS n -> if n Prelude.== 0 then fO () else fS (n Prelude.- 1))
+      (\_ ->
+      case v0 of {
+       LinearScan__V__Coq_nil -> LinearScan__V__Coq_cons a (Prelude.succ 0)
+        (LinearScan__V__Coq_cons a 0 LinearScan__V__Coq_nil);
+       LinearScan__V__Coq_cons h n1 t ->
+        unsafeCoerce (\_ -> Prelude.error "absurd case")})
+      (\nn' -> LinearScan__V__Coq_cons a (Prelude.succ (Prelude.succ nn'))
+      (_LinearScan__V__shiftrepeat nn' v0))
+      n0}
+
+_LinearScan__V__trunc :: Prelude.Int -> Prelude.Int -> (LinearScan__V__Coq_t
+                         a1) -> LinearScan__V__Coq_t a1
+_LinearScan__V__trunc n p x =
+  Datatypes.nat_rect (\_ v -> Logic.eq_rect n v (Peano.minus n 0))
+    (\p0 f _ v ->
+    _LinearScan__V__shiftout (Peano.minus n (Prelude.succ p0))
+      (Logic.eq_rect_r (Peano.minus (Prelude.succ n) (Prelude.succ p0))
+        (f __ v) (Prelude.succ (Peano.minus n (Prelude.succ p0))))) p __ x
+
+_LinearScan__V__append :: Prelude.Int -> Prelude.Int -> (LinearScan__V__Coq_t
+                          a1) -> (LinearScan__V__Coq_t a1) ->
+                          LinearScan__V__Coq_t a1
+_LinearScan__V__append n p v w =
+  case v of {
+   LinearScan__V__Coq_nil -> w;
+   LinearScan__V__Coq_cons a n0 v' -> LinearScan__V__Coq_cons a
+    ((Prelude.+) n0 p) (_LinearScan__V__append n0 p v' w)}
+
+_LinearScan__V__rev_append_tail :: Prelude.Int -> Prelude.Int ->
+                                   (LinearScan__V__Coq_t a1) ->
+                                   (LinearScan__V__Coq_t a1) ->
+                                   LinearScan__V__Coq_t a1
+_LinearScan__V__rev_append_tail n p v w =
+  case v of {
+   LinearScan__V__Coq_nil -> w;
+   LinearScan__V__Coq_cons a n0 v' ->
+    _LinearScan__V__rev_append_tail n0 (Prelude.succ p) v'
+      (LinearScan__V__Coq_cons a p w)}
+
+_LinearScan__V__rev_append :: Prelude.Int -> Prelude.Int ->
+                              (LinearScan__V__Coq_t a1) ->
+                              (LinearScan__V__Coq_t a1) ->
+                              LinearScan__V__Coq_t a1
+_LinearScan__V__rev_append n p v w =
+  Logic.eq_rect_r (Plus.tail_plus n p)
+    (_LinearScan__V__rev_append_tail n p v w) ((Prelude.+) n p)
+
+_LinearScan__V__rev :: Prelude.Int -> (LinearScan__V__Coq_t a1) ->
+                       LinearScan__V__Coq_t a1
+_LinearScan__V__rev n v =
+  Logic.eq_rect_r ((Prelude.+) n 0)
+    (_LinearScan__V__rev_append n 0 v LinearScan__V__Coq_nil) n
+
+_LinearScan__V__map :: (a1 -> a2) -> Prelude.Int -> (LinearScan__V__Coq_t 
+                       a1) -> LinearScan__V__Coq_t a2
+_LinearScan__V__map f n v =
+  case v of {
+   LinearScan__V__Coq_nil -> LinearScan__V__Coq_nil;
+   LinearScan__V__Coq_cons a n0 v' -> LinearScan__V__Coq_cons (f a) n0
+    (_LinearScan__V__map f n0 v')}
+
+_LinearScan__V__map2 :: (a1 -> a2 -> a3) -> Prelude.Int ->
+                        (LinearScan__V__Coq_t a1) -> (LinearScan__V__Coq_t
+                        a2) -> LinearScan__V__Coq_t a3
+_LinearScan__V__map2 g n v1 v2 =
+  case v1 of {
+   LinearScan__V__Coq_nil ->
+    case v2 of {
+     LinearScan__V__Coq_nil -> LinearScan__V__Coq_nil;
+     LinearScan__V__Coq_cons h n0 t ->
+      unsafeCoerce (\_ -> Prelude.error "absurd case")};
+   LinearScan__V__Coq_cons h1 n0 t1 ->
+    case v2 of {
+     LinearScan__V__Coq_nil -> Prelude.error "absurd case";
+     LinearScan__V__Coq_cons h2 n1 t2 -> LinearScan__V__Coq_cons (g h1 h2) n1
+      (_LinearScan__V__map2 g n1 t1 t2)}}
+
+_LinearScan__V__fold_left :: (a2 -> a1 -> a2) -> a2 -> Prelude.Int ->
+                             (LinearScan__V__Coq_t a1) -> a2
+_LinearScan__V__fold_left f b n v =
+  case v of {
+   LinearScan__V__Coq_nil -> b;
+   LinearScan__V__Coq_cons a n0 w -> _LinearScan__V__fold_left f (f b a) n0 w}
+
+_LinearScan__V__fold_right :: (a1 -> a2 -> a2) -> Prelude.Int ->
+                              (LinearScan__V__Coq_t a1) -> a2 -> a2
+_LinearScan__V__fold_right f n v b =
+  case v of {
+   LinearScan__V__Coq_nil -> b;
+   LinearScan__V__Coq_cons a n0 w ->
+    f a (_LinearScan__V__fold_right f n0 w b)}
+
+_LinearScan__V__fold_right2 :: (a1 -> a2 -> a3 -> a3) -> Prelude.Int ->
+                               (LinearScan__V__Coq_t a1) ->
+                               (LinearScan__V__Coq_t a2) -> a3 -> a3
+_LinearScan__V__fold_right2 g n v w c =
+  case v of {
+   LinearScan__V__Coq_nil ->
+    case w of {
+     LinearScan__V__Coq_nil -> c;
+     LinearScan__V__Coq_cons h n0 t ->
+      unsafeCoerce (\_ -> Prelude.error "absurd case")};
+   LinearScan__V__Coq_cons h1 n0 t1 ->
+    case w of {
+     LinearScan__V__Coq_nil -> Prelude.error "absurd case";
+     LinearScan__V__Coq_cons h2 n1 t2 ->
+      g h1 h2 (_LinearScan__V__fold_right2 g n1 t1 t2 c)}}
+
+_LinearScan__V__fold_left2 :: (a1 -> a2 -> a3 -> a1) -> a1 -> Prelude.Int ->
+                              (LinearScan__V__Coq_t a2) ->
+                              (LinearScan__V__Coq_t a3) -> a1
+_LinearScan__V__fold_left2 f a n v w =
+  case v of {
+   LinearScan__V__Coq_nil ->
+    case w of {
+     LinearScan__V__Coq_nil -> a;
+     LinearScan__V__Coq_cons h n0 t -> unsafeCoerce (\_ -> Datatypes.id)};
+   LinearScan__V__Coq_cons vh vn vt ->
+    case w of {
+     LinearScan__V__Coq_nil -> unsafeCoerce (\_ -> Datatypes.id) vt;
+     LinearScan__V__Coq_cons wh n0 wt ->
+      _LinearScan__V__fold_left2 f (f a vh wh) n0 vt wt}}
+
+_LinearScan__V__of_list :: ([] a1) -> LinearScan__V__Coq_t a1
+_LinearScan__V__of_list l =
+  case l of {
+   [] -> LinearScan__V__Coq_nil;
+   (:) h tail -> LinearScan__V__Coq_cons h (Datatypes.length tail)
+    (_LinearScan__V__of_list tail)}
+
+_LinearScan__V__to_list :: Prelude.Int -> (LinearScan__V__Coq_t a1) -> [] a1
+_LinearScan__V__to_list n v =
+  let {
+   fold_right_fix n0 v0 b =
+     case v0 of {
+      LinearScan__V__Coq_nil -> b;
+      LinearScan__V__Coq_cons a n1 w -> (:) a (fold_right_fix n1 w b)}}
+  in fold_right_fix n v []
+
+type LinearScan__Vec a = LinearScan__V__Coq_t a
+
 data LinearScan__ScanStateDesc =
    LinearScan__Build_ScanStateDesc Prelude.Int ([] Fin0.Coq_fin) ([]
                                                                  Fin0.Coq_fin) 
- ([] Fin0.Coq_fin) ([] Fin0.Coq_fin) (Fin0.Coq_fin -> Interval.IntervalDesc) 
- (Fin0.Coq_fin -> Prelude.Maybe LinearScan__PhysReg) (LinearScan__PhysReg ->
-                                                     Prelude.Maybe
-                                                     Interval.IntervalDesc)
+ ([] Fin0.Coq_fin) ([] Fin0.Coq_fin) (LinearScan__Vec Interval.IntervalDesc) 
+ (LinearScan__Vec (Prelude.Maybe LinearScan__PhysReg)) (LinearScan__Vec
+                                                       (Prelude.Maybe
+                                                       Interval.IntervalDesc))
 
 _LinearScan__coq_ScanStateDesc_rect :: (Prelude.Int -> ([] Fin0.Coq_fin) ->
                                        ([] Fin0.Coq_fin) -> ([] Fin0.Coq_fin)
-                                       -> ([] Fin0.Coq_fin) -> (Fin0.Coq_fin
-                                       -> Interval.IntervalDesc) ->
-                                       (Fin0.Coq_fin -> Prelude.Maybe
-                                       LinearScan__PhysReg) ->
-                                       (LinearScan__PhysReg -> Prelude.Maybe
-                                       Interval.IntervalDesc) -> () -> a1) ->
+                                       -> ([] Fin0.Coq_fin) ->
+                                       (LinearScan__Vec
+                                       Interval.IntervalDesc) ->
+                                       (LinearScan__Vec
+                                       (Prelude.Maybe LinearScan__PhysReg))
+                                       -> (LinearScan__Vec
+                                       (Prelude.Maybe Interval.IntervalDesc))
+                                       -> () -> a1) ->
                                        LinearScan__ScanStateDesc -> a1
 _LinearScan__coq_ScanStateDesc_rect f s =
   case s of {
@@ -58,12 +391,13 @@ _LinearScan__coq_ScanStateDesc_rect f s =
 
 _LinearScan__coq_ScanStateDesc_rec :: (Prelude.Int -> ([] Fin0.Coq_fin) ->
                                       ([] Fin0.Coq_fin) -> ([] Fin0.Coq_fin)
-                                      -> ([] Fin0.Coq_fin) -> (Fin0.Coq_fin
-                                      -> Interval.IntervalDesc) ->
-                                      (Fin0.Coq_fin -> Prelude.Maybe
-                                      LinearScan__PhysReg) ->
-                                      (LinearScan__PhysReg -> Prelude.Maybe
-                                      Interval.IntervalDesc) -> () -> a1) ->
+                                      -> ([] Fin0.Coq_fin) ->
+                                      (LinearScan__Vec Interval.IntervalDesc)
+                                      -> (LinearScan__Vec
+                                      (Prelude.Maybe LinearScan__PhysReg)) ->
+                                      (LinearScan__Vec
+                                      (Prelude.Maybe Interval.IntervalDesc))
+                                      -> () -> a1) ->
                                       LinearScan__ScanStateDesc -> a1
 _LinearScan__coq_ScanStateDesc_rec =
   _LinearScan__coq_ScanStateDesc_rect
@@ -72,7 +406,7 @@ _LinearScan__nextInterval :: LinearScan__ScanStateDesc -> Prelude.Int
 _LinearScan__nextInterval s =
   case s of {
    LinearScan__Build_ScanStateDesc nextInterval0 unhandled0 active0 inactive0
-    handled0 getInterval0 assignments0 getFixedInterval0 -> nextInterval0}
+    handled0 intervals0 assignments0 fixedIntervals0 -> nextInterval0}
 
 type LinearScan__IntervalId = Fin0.Coq_fin
 
@@ -81,50 +415,48 @@ _LinearScan__unhandled :: LinearScan__ScanStateDesc -> []
 _LinearScan__unhandled s =
   case s of {
    LinearScan__Build_ScanStateDesc nextInterval0 unhandled0 active0 inactive0
-    handled0 getInterval0 assignments0 getFixedInterval0 -> unhandled0}
+    handled0 intervals0 assignments0 fixedIntervals0 -> unhandled0}
 
 _LinearScan__active :: LinearScan__ScanStateDesc -> [] LinearScan__IntervalId
 _LinearScan__active s =
   case s of {
    LinearScan__Build_ScanStateDesc nextInterval0 unhandled0 active0 inactive0
-    handled0 getInterval0 assignments0 getFixedInterval0 -> active0}
+    handled0 intervals0 assignments0 fixedIntervals0 -> active0}
 
 _LinearScan__inactive :: LinearScan__ScanStateDesc -> []
                          LinearScan__IntervalId
 _LinearScan__inactive s =
   case s of {
    LinearScan__Build_ScanStateDesc nextInterval0 unhandled0 active0 inactive0
-    handled0 getInterval0 assignments0 getFixedInterval0 -> inactive0}
+    handled0 intervals0 assignments0 fixedIntervals0 -> inactive0}
 
 _LinearScan__handled :: LinearScan__ScanStateDesc -> []
                         LinearScan__IntervalId
 _LinearScan__handled s =
   case s of {
    LinearScan__Build_ScanStateDesc nextInterval0 unhandled0 active0 inactive0
-    handled0 getInterval0 assignments0 getFixedInterval0 -> handled0}
+    handled0 intervals0 assignments0 fixedIntervals0 -> handled0}
 
-_LinearScan__getInterval :: LinearScan__ScanStateDesc ->
-                            LinearScan__IntervalId -> Interval.IntervalDesc
-_LinearScan__getInterval s =
+_LinearScan__intervals :: LinearScan__ScanStateDesc -> LinearScan__Vec
+                          Interval.IntervalDesc
+_LinearScan__intervals s =
   case s of {
    LinearScan__Build_ScanStateDesc nextInterval0 unhandled0 active0 inactive0
-    handled0 getInterval0 assignments0 getFixedInterval0 -> getInterval0}
+    handled0 intervals0 assignments0 fixedIntervals0 -> intervals0}
 
-_LinearScan__assignments :: LinearScan__ScanStateDesc ->
-                            LinearScan__IntervalId -> Prelude.Maybe
-                            LinearScan__PhysReg
+_LinearScan__assignments :: LinearScan__ScanStateDesc -> LinearScan__Vec
+                            (Prelude.Maybe LinearScan__PhysReg)
 _LinearScan__assignments s =
   case s of {
    LinearScan__Build_ScanStateDesc nextInterval0 unhandled0 active0 inactive0
-    handled0 getInterval0 assignments0 getFixedInterval0 -> assignments0}
+    handled0 intervals0 assignments0 fixedIntervals0 -> assignments0}
 
-_LinearScan__getFixedInterval :: LinearScan__ScanStateDesc ->
-                                 LinearScan__PhysReg -> Prelude.Maybe
-                                 Interval.IntervalDesc
-_LinearScan__getFixedInterval s =
+_LinearScan__fixedIntervals :: LinearScan__ScanStateDesc -> LinearScan__Vec
+                               (Prelude.Maybe Interval.IntervalDesc)
+_LinearScan__fixedIntervals s =
   case s of {
    LinearScan__Build_ScanStateDesc nextInterval0 unhandled0 active0 inactive0
-    handled0 getInterval0 assignments0 getFixedInterval0 -> getFixedInterval0}
+    handled0 intervals0 assignments0 fixedIntervals0 -> fixedIntervals0}
 
 _LinearScan__all_state_lists :: LinearScan__ScanStateDesc -> []
                                 LinearScan__IntervalId
@@ -145,10 +477,10 @@ _LinearScan__transportId sd sd' x =
    Specif.Coq_left ->
     case sd of {
      LinearScan__Build_ScanStateDesc nextInterval0 unhandled0 active0
-      inactive0 handled0 getInterval0 assignments0 getFixedInterval0 ->
+      inactive0 handled0 intervals0 assignments0 fixedIntervals0 ->
       case sd' of {
        LinearScan__Build_ScanStateDesc nextInterval1 unhandled1 active1
-        inactive1 handled1 getInterval1 assignments1 getFixedInterval1 ->
+        inactive1 handled1 intervals1 assignments1 fixedIntervals1 ->
         let {h0 = Lib.lt_sub nextInterval0 nextInterval1} in
         Logic.eq_rec ((Prelude.+) h0 nextInterval0)
           (Fin.coq_R nextInterval0 h0 x) nextInterval1}};
@@ -162,12 +494,19 @@ _LinearScan__unhandledExtent sd =
    [] -> 0;
    (:) i l ->
     case l of {
-     [] -> Interval.intervalExtent ( (_LinearScan__getInterval sd i));
+     [] ->
+      Interval.intervalExtent
+        (
+          (_LinearScan__V__nth (_LinearScan__nextInterval sd)
+            (_LinearScan__intervals sd) i));
      (:) i0 l0 ->
       let {
        f = \n x ->
         (Prelude.+) n
-          (Interval.intervalExtent ( (_LinearScan__getInterval sd x)))}
+          (Interval.intervalExtent
+            (
+              (_LinearScan__V__nth (_LinearScan__nextInterval sd)
+                (_LinearScan__intervals sd) x)))}
       in
       (\f -> Prelude.flip (Data.List.foldl' f)) f ((:) i ((:) i0 l0)) 0}}
 
@@ -191,7 +530,8 @@ _LinearScan__curId sd =
 _LinearScan__curIntDetails :: LinearScan__ScanStateDesc ->
                               Interval.IntervalDesc
 _LinearScan__curIntDetails sd =
-  _LinearScan__getInterval sd (_LinearScan__curId sd)
+  _LinearScan__V__nth (_LinearScan__nextInterval sd)
+    (_LinearScan__intervals sd) (_LinearScan__curId sd)
 
 _LinearScan__curIntDesc :: LinearScan__ScanStateDesc -> Interval.IntervalDesc
 _LinearScan__curIntDesc sd =
@@ -289,14 +629,13 @@ _LinearScan__moveUnhandledToActive :: LinearScan__ScanStateDesc ->
 _LinearScan__moveUnhandledToActive sd reg =
   case sd of {
    LinearScan__Build_ScanStateDesc nextInterval0 unhandled0 active0 inactive0
-    handled0 getInterval0 assignments0 getFixedInterval0 ->
+    handled0 intervals0 assignments0 fixedIntervals0 ->
     case unhandled0 of {
      [] -> Logic.coq_False_rec;
      (:) i unhandled1 -> LinearScan__Build_ScanStateDesc nextInterval0
-      unhandled1 ((:) i active0) inactive0 handled0 getInterval0 (\i0 ->
-      case Compare.cmp_eq_dec (Fin0.fin_CompareSpec nextInterval0) i0 i of {
-       Specif.Coq_left -> Prelude.Just reg;
-       Specif.Coq_right -> assignments0 i0}) getFixedInterval0}}
+      unhandled1 ((:) i active0) inactive0 handled0 intervals0
+      (_LinearScan__V__replace nextInterval0 assignments0 i (Prelude.Just
+        reg)) fixedIntervals0}}
 
 _LinearScan__moveActiveToHandled :: LinearScan__ScanStateDesc ->
                                     LinearScan__IntervalId ->
@@ -308,8 +647,8 @@ _LinearScan__moveActiveToHandled sd x =
       (Compare.cmp_eq_dec
         (Fin0.fin_CompareSpec (_LinearScan__nextInterval sd))) x
       (_LinearScan__active sd)) ((:) x (_LinearScan__inactive sd))
-    (_LinearScan__handled sd) (_LinearScan__getInterval sd)
-    (_LinearScan__assignments sd) (_LinearScan__getFixedInterval sd)
+    (_LinearScan__handled sd) (_LinearScan__intervals sd)
+    (_LinearScan__assignments sd) (_LinearScan__fixedIntervals sd)
 
 _LinearScan__moveActiveToInactive :: LinearScan__ScanStateDesc ->
                                      LinearScan__IntervalId ->
@@ -321,8 +660,8 @@ _LinearScan__moveActiveToInactive sd x =
       (Compare.cmp_eq_dec
         (Fin0.fin_CompareSpec (_LinearScan__nextInterval sd))) x
       (_LinearScan__active sd)) ((:) x (_LinearScan__inactive sd))
-    (_LinearScan__handled sd) (_LinearScan__getInterval sd)
-    (_LinearScan__assignments sd) (_LinearScan__getFixedInterval sd)
+    (_LinearScan__handled sd) (_LinearScan__intervals sd)
+    (_LinearScan__assignments sd) (_LinearScan__fixedIntervals sd)
 
 _LinearScan__moveInactiveToActive :: LinearScan__ScanStateDesc ->
                                      LinearScan__IntervalId ->
@@ -334,8 +673,8 @@ _LinearScan__moveInactiveToActive sd x =
       (Compare.cmp_eq_dec
         (Fin0.fin_CompareSpec (_LinearScan__nextInterval sd))) x
       (_LinearScan__inactive sd)) (_LinearScan__handled sd)
-    (_LinearScan__getInterval sd) (_LinearScan__assignments sd)
-    (_LinearScan__getFixedInterval sd)
+    (_LinearScan__intervals sd) (_LinearScan__assignments sd)
+    (_LinearScan__fixedIntervals sd)
 
 _LinearScan__moveInactiveToHandled :: LinearScan__ScanStateDesc ->
                                       LinearScan__IntervalId ->
@@ -347,343 +686,83 @@ _LinearScan__moveInactiveToHandled sd x =
       (Compare.cmp_eq_dec
         (Fin0.fin_CompareSpec (_LinearScan__nextInterval sd))) x
       (_LinearScan__inactive sd)) ((:) x (_LinearScan__handled sd))
-    (_LinearScan__getInterval sd) (_LinearScan__assignments sd)
-    (_LinearScan__getFixedInterval sd)
-
-_LinearScan__nextIntersectionWith :: Interval.IntervalDesc ->
-                                     LinearScan__ScanStateDesc ->
-                                     LinearScan__IntervalId -> Prelude.Maybe
-                                     Prelude.Int
-_LinearScan__nextIntersectionWith d sd jid =
-  Interval.firstIntersectionPoint ( (_LinearScan__getInterval sd jid)) d
-
-_LinearScan__getRegisterIndex :: LinearScan__ScanStateDesc ->
-                                 (LinearScan__IntervalId -> Prelude.Maybe
-                                 Prelude.Int) -> (LinearScan__PhysReg ->
-                                 Prelude.Maybe Prelude.Int) -> ([]
-                                 LinearScan__IntervalId) ->
-                                 LinearScan__PhysReg -> Prelude.Maybe
-                                 Prelude.Int
-_LinearScan__getRegisterIndex sd intervalIndex registerIndex intervals =
-  Prelude.foldr (\x f r ->
-    case _LinearScan__assignments sd x of {
-     Prelude.Just a ->
-      case Compare.cmp_eq_dec (Fin0.fin_CompareSpec _LinearScan__maxReg) a r of {
-       Specif.Coq_left -> intervalIndex x;
-       Specif.Coq_right -> f r};
-     Prelude.Nothing -> f r}) registerIndex intervals
-
-_LinearScan__findRegister_F :: ((LinearScan__PhysReg -> Prelude.Maybe
-                               Prelude.Int) -> LinearScan__PhysReg -> (,)
-                               LinearScan__PhysReg
-                               (Prelude.Maybe Prelude.Int)) ->
-                               (LinearScan__PhysReg -> Prelude.Maybe
-                               Prelude.Int) -> LinearScan__PhysReg -> (,)
-                               LinearScan__PhysReg
-                               (Prelude.Maybe Prelude.Int)
-_LinearScan__findRegister_F findRegister0 registerIndex start =
-  case registerIndex start of {
-   Prelude.Just pos ->
-    case Fin0.pred_fin _LinearScan__maxReg start of {
-     Prelude.Just nreg ->
-      case findRegister0 registerIndex nreg of {
-       (,) reg o ->
-        case o of {
-         Prelude.Just pos' ->
-          case NPeano.ltb pos pos' of {
-           Prelude.True -> (,) reg (Prelude.Just pos');
-           Prelude.False -> (,) reg (Prelude.Just pos)};
-         Prelude.Nothing -> (,) reg Prelude.Nothing}};
-     Prelude.Nothing -> (,) start (Prelude.Just pos)};
-   Prelude.Nothing -> (,) start Prelude.Nothing}
-
-_LinearScan__findRegister_terminate :: (LinearScan__PhysReg -> Prelude.Maybe
-                                       Prelude.Int) -> LinearScan__PhysReg ->
-                                       ((,) LinearScan__PhysReg
-                                       (Prelude.Maybe Prelude.Int))
-_LinearScan__findRegister_terminate registerIndex start =
-  case registerIndex start of {
-   Prelude.Just pos ->
-    case Fin0.pred_fin _LinearScan__maxReg start of {
-     Prelude.Just nreg ->
-      Specif.sig_rec (\rec_res _ ->
-        case rec_res of {
-         (,) reg o ->
-          case o of {
-           Prelude.Just pos' ->
-            case NPeano.ltb pos pos' of {
-             Prelude.True -> (,) reg (Prelude.Just pos');
-             Prelude.False -> (,) reg (Prelude.Just pos)};
-           Prelude.Nothing -> (,) reg Prelude.Nothing}})
-        (_LinearScan__findRegister_terminate registerIndex nreg);
-     Prelude.Nothing -> (,) start (Prelude.Just pos)};
-   Prelude.Nothing -> (,) start Prelude.Nothing}
-
-_LinearScan__findRegister :: (LinearScan__PhysReg -> Prelude.Maybe
-                             Prelude.Int) -> LinearScan__PhysReg -> (,)
-                             LinearScan__PhysReg (Prelude.Maybe Prelude.Int)
-_LinearScan__findRegister registerIndex start =
-  case registerIndex start of {
-   Prelude.Just pos ->
-    case Fin0.pred_fin _LinearScan__maxReg start of {
-     Prelude.Just nreg ->
-      Specif.sig_rec (\rec_res _ ->
-        case rec_res of {
-         (,) reg o ->
-          case o of {
-           Prelude.Just pos' ->
-            case NPeano.ltb pos pos' of {
-             Prelude.True -> (,) reg (Prelude.Just pos');
-             Prelude.False -> (,) reg (Prelude.Just pos)};
-           Prelude.Nothing -> (,) reg Prelude.Nothing}})
-        (_LinearScan__findRegister registerIndex nreg);
-     Prelude.Nothing -> (,) start (Prelude.Just pos)};
-   Prelude.Nothing -> (,) start Prelude.Nothing}
-
-data LinearScan__R_findRegister =
-   LinearScan__R_findRegister_0 LinearScan__PhysReg
- | LinearScan__R_findRegister_1 LinearScan__PhysReg Prelude.Int
- | LinearScan__R_findRegister_2 LinearScan__PhysReg Prelude.Int Fin0.Coq_fin 
- ((,) LinearScan__PhysReg (Prelude.Maybe Prelude.Int)) LinearScan__R_findRegister 
- LinearScan__PhysReg
- | LinearScan__R_findRegister_3 LinearScan__PhysReg Prelude.Int Fin0.Coq_fin 
- ((,) LinearScan__PhysReg (Prelude.Maybe Prelude.Int)) LinearScan__R_findRegister 
- LinearScan__PhysReg Prelude.Int
- | LinearScan__R_findRegister_4 LinearScan__PhysReg Prelude.Int Fin0.Coq_fin 
- ((,) LinearScan__PhysReg (Prelude.Maybe Prelude.Int)) LinearScan__R_findRegister 
- LinearScan__PhysReg Prelude.Int
-
-_LinearScan__coq_R_findRegister_rect :: (LinearScan__PhysReg -> Prelude.Maybe
-                                        Prelude.Int) -> (LinearScan__PhysReg
-                                        -> () -> a1) -> (LinearScan__PhysReg
-                                        -> Prelude.Int -> () -> () -> a1) ->
-                                        (LinearScan__PhysReg -> Prelude.Int
-                                        -> () -> Fin0.Coq_fin -> () -> ((,)
-                                        LinearScan__PhysReg
-                                        (Prelude.Maybe Prelude.Int)) ->
-                                        LinearScan__R_findRegister -> a1 ->
-                                        LinearScan__PhysReg -> () -> a1) ->
-                                        (LinearScan__PhysReg -> Prelude.Int
-                                        -> () -> Fin0.Coq_fin -> () -> ((,)
-                                        LinearScan__PhysReg
-                                        (Prelude.Maybe Prelude.Int)) ->
-                                        LinearScan__R_findRegister -> a1 ->
-                                        LinearScan__PhysReg -> Prelude.Int ->
-                                        () -> () -> a1) ->
-                                        (LinearScan__PhysReg -> Prelude.Int
-                                        -> () -> Fin0.Coq_fin -> () -> ((,)
-                                        LinearScan__PhysReg
-                                        (Prelude.Maybe Prelude.Int)) ->
-                                        LinearScan__R_findRegister -> a1 ->
-                                        LinearScan__PhysReg -> Prelude.Int ->
-                                        () -> () -> a1) ->
-                                        LinearScan__PhysReg -> ((,)
-                                        LinearScan__PhysReg
-                                        (Prelude.Maybe Prelude.Int)) ->
-                                        LinearScan__R_findRegister -> a1
-_LinearScan__coq_R_findRegister_rect registerIndex f f0 f1 f2 f3 start p r =
-  case r of {
-   LinearScan__R_findRegister_0 start0 -> f start0 __;
-   LinearScan__R_findRegister_1 start0 pos -> f0 start0 pos __ __;
-   LinearScan__R_findRegister_2 start0 pos nreg res r0 reg ->
-    f1 start0 pos __ nreg __ res r0
-      (_LinearScan__coq_R_findRegister_rect registerIndex f f0 f1 f2 f3 nreg
-        res r0) reg __;
-   LinearScan__R_findRegister_3 start0 pos nreg res r0 reg pos' ->
-    f2 start0 pos __ nreg __ res r0
-      (_LinearScan__coq_R_findRegister_rect registerIndex f f0 f1 f2 f3 nreg
-        res r0) reg pos' __ __;
-   LinearScan__R_findRegister_4 start0 pos nreg res r0 reg pos' ->
-    f3 start0 pos __ nreg __ res r0
-      (_LinearScan__coq_R_findRegister_rect registerIndex f f0 f1 f2 f3 nreg
-        res r0) reg pos' __ __}
-
-_LinearScan__coq_R_findRegister_rec :: (LinearScan__PhysReg -> Prelude.Maybe
-                                       Prelude.Int) -> (LinearScan__PhysReg
-                                       -> () -> a1) -> (LinearScan__PhysReg
-                                       -> Prelude.Int -> () -> () -> a1) ->
-                                       (LinearScan__PhysReg -> Prelude.Int ->
-                                       () -> Fin0.Coq_fin -> () -> ((,)
-                                       LinearScan__PhysReg
-                                       (Prelude.Maybe Prelude.Int)) ->
-                                       LinearScan__R_findRegister -> a1 ->
-                                       LinearScan__PhysReg -> () -> a1) ->
-                                       (LinearScan__PhysReg -> Prelude.Int ->
-                                       () -> Fin0.Coq_fin -> () -> ((,)
-                                       LinearScan__PhysReg
-                                       (Prelude.Maybe Prelude.Int)) ->
-                                       LinearScan__R_findRegister -> a1 ->
-                                       LinearScan__PhysReg -> Prelude.Int ->
-                                       () -> () -> a1) ->
-                                       (LinearScan__PhysReg -> Prelude.Int ->
-                                       () -> Fin0.Coq_fin -> () -> ((,)
-                                       LinearScan__PhysReg
-                                       (Prelude.Maybe Prelude.Int)) ->
-                                       LinearScan__R_findRegister -> a1 ->
-                                       LinearScan__PhysReg -> Prelude.Int ->
-                                       () -> () -> a1) -> LinearScan__PhysReg
-                                       -> ((,) LinearScan__PhysReg
-                                       (Prelude.Maybe Prelude.Int)) ->
-                                       LinearScan__R_findRegister -> a1
-_LinearScan__coq_R_findRegister_rec registerIndex =
-  _LinearScan__coq_R_findRegister_rect registerIndex
-
-_LinearScan__findRegister_rect :: (LinearScan__PhysReg -> Prelude.Maybe
-                                  Prelude.Int) -> (LinearScan__PhysReg -> ()
-                                  -> a1) -> (LinearScan__PhysReg ->
-                                  Prelude.Int -> () -> () -> a1) ->
-                                  (LinearScan__PhysReg -> Prelude.Int -> ()
-                                  -> Fin0.Coq_fin -> () -> a1 ->
-                                  LinearScan__PhysReg -> () -> a1) ->
-                                  (LinearScan__PhysReg -> Prelude.Int -> ()
-                                  -> Fin0.Coq_fin -> () -> a1 ->
-                                  LinearScan__PhysReg -> Prelude.Int -> () ->
-                                  () -> a1) -> (LinearScan__PhysReg ->
-                                  Prelude.Int -> () -> Fin0.Coq_fin -> () ->
-                                  a1 -> LinearScan__PhysReg -> Prelude.Int ->
-                                  () -> () -> a1) -> LinearScan__PhysReg ->
-                                  a1
-_LinearScan__findRegister_rect registerIndex f f0 f1 f2 f3 start =
-  Logic.eq_rect_r
-    (case registerIndex start of {
-      Prelude.Just pos ->
-       case Fin0.pred_fin _LinearScan__maxReg start of {
-        Prelude.Just nreg ->
-         case _LinearScan__findRegister registerIndex nreg of {
-          (,) reg o ->
-           case o of {
-            Prelude.Just pos' ->
-             case NPeano.ltb pos pos' of {
-              Prelude.True -> (,) reg (Prelude.Just pos');
-              Prelude.False -> (,) reg (Prelude.Just pos)};
-            Prelude.Nothing -> (,) reg Prelude.Nothing}};
-        Prelude.Nothing -> (,) start (Prelude.Just pos)};
-      Prelude.Nothing -> (,) start Prelude.Nothing})
-    (let {f4 = f3 start} in
-     let {f5 = f2 start} in
-     let {f6 = f1 start} in
-     let {f7 = f0 start} in
-     let {f8 = f start} in
-     case registerIndex start of {
-      Prelude.Just n ->
-       let {f9 = f7 n __} in
-       let {f10 = f6 n __} in
-       let {f11 = f5 n __} in
-       let {f12 = f4 n __} in
-       case Fin0.pred_fin _LinearScan__maxReg start of {
-        Prelude.Just f13 ->
-         let {f14 = f12 f13 __} in
-         let {f15 = f11 f13 __} in
-         let {f16 = f10 f13 __} in
-         case _LinearScan__findRegister registerIndex f13 of {
-          (,) p o ->
-           case o of {
-            Prelude.Just n0 ->
-             let {f17 = \h -> f14 h p n0 __} in
-             let {f18 = \h -> f15 h p n0 __} in
-             case NPeano.ltb n n0 of {
-              Prelude.True ->
-               let {f19 = \h -> f18 h __} in
-               let {
-                hrec = Logic.eq_rect o
-                         (Logic.eq_rect
-                           (_LinearScan__findRegister registerIndex f13)
-                           (_LinearScan__findRegister_rect registerIndex f f0
-                             f1 f2 f3 f13) ((,) p o)) (Prelude.Just n0)}
-               in
-               f19 hrec;
-              Prelude.False ->
-               let {f19 = \h -> f17 h __} in
-               let {
-                hrec = Logic.eq_rect o
-                         (Logic.eq_rect
-                           (_LinearScan__findRegister registerIndex f13)
-                           (_LinearScan__findRegister_rect registerIndex f f0
-                             f1 f2 f3 f13) ((,) p o)) (Prelude.Just n0)}
-               in
-               f19 hrec};
-            Prelude.Nothing ->
-             let {f17 = \h -> f16 h p __} in
-             let {
-              hrec = Logic.eq_rect o
-                       (Logic.eq_rect
-                         (_LinearScan__findRegister registerIndex f13)
-                         (_LinearScan__findRegister_rect registerIndex f f0
-                           f1 f2 f3 f13) ((,) p o)) Prelude.Nothing}
-             in
-             f17 hrec}};
-        Prelude.Nothing -> f9 __};
-      Prelude.Nothing -> f8 __})
-    (_LinearScan__findRegister registerIndex start)
-
-_LinearScan__findRegister_rec :: (LinearScan__PhysReg -> Prelude.Maybe
-                                 Prelude.Int) -> (LinearScan__PhysReg -> ()
-                                 -> a1) -> (LinearScan__PhysReg ->
-                                 Prelude.Int -> () -> () -> a1) ->
-                                 (LinearScan__PhysReg -> Prelude.Int -> () ->
-                                 Fin0.Coq_fin -> () -> a1 ->
-                                 LinearScan__PhysReg -> () -> a1) ->
-                                 (LinearScan__PhysReg -> Prelude.Int -> () ->
-                                 Fin0.Coq_fin -> () -> a1 ->
-                                 LinearScan__PhysReg -> Prelude.Int -> () ->
-                                 () -> a1) -> (LinearScan__PhysReg ->
-                                 Prelude.Int -> () -> Fin0.Coq_fin -> () ->
-                                 a1 -> LinearScan__PhysReg -> Prelude.Int ->
-                                 () -> () -> a1) -> LinearScan__PhysReg -> a1
-_LinearScan__findRegister_rec registerIndex =
-  _LinearScan__findRegister_rect registerIndex
-
-_LinearScan__coq_R_findRegister_correct :: (LinearScan__PhysReg ->
-                                           Prelude.Maybe Prelude.Int) ->
-                                           LinearScan__PhysReg -> ((,)
-                                           LinearScan__PhysReg
-                                           (Prelude.Maybe Prelude.Int)) ->
-                                           LinearScan__R_findRegister
-_LinearScan__coq_R_findRegister_correct x x0 res =
-  _LinearScan__findRegister_rect x (\y _ z _ ->
-    Logic.eq_rec_r ((,) y Prelude.Nothing) (LinearScan__R_findRegister_0 y) z)
-    (\y y0 _ _ z _ ->
-    Logic.eq_rec_r ((,) y (Prelude.Just y0)) (LinearScan__R_findRegister_1 y
-      y0) z) (\y y0 _ y2 _ y4 y5 _ z _ ->
-    Logic.eq_rec_r ((,) y5 Prelude.Nothing) (LinearScan__R_findRegister_2 y
-      y0 y2 (_LinearScan__findRegister x y2)
-      (y4 (_LinearScan__findRegister x y2) __) y5) z)
-    (\y y0 _ y2 _ y4 y5 y6 _ _ z _ ->
-    Logic.eq_rec_r ((,) y5 (Prelude.Just y6)) (LinearScan__R_findRegister_3 y
-      y0 y2 (_LinearScan__findRegister x y2)
-      (y4 (_LinearScan__findRegister x y2) __) y5 y6) z)
-    (\y y0 _ y2 _ y4 y5 y6 _ _ z _ ->
-    Logic.eq_rec_r ((,) y5 (Prelude.Just y0)) (LinearScan__R_findRegister_4 y
-      y0 y2 (_LinearScan__findRegister x y2)
-      (y4 (_LinearScan__findRegister x y2) __) y5 y6) z) x0 res __
+    (_LinearScan__intervals sd) (_LinearScan__assignments sd)
+    (_LinearScan__fixedIntervals sd)
 
 _LinearScan__splitInterval :: LinearScan__ScanStateDesc -> (Prelude.Maybe
                               Prelude.Int) -> LinearScan__NextState
 _LinearScan__splitInterval sd before =
   sd
 
+_LinearScan__atRegister :: LinearScan__ScanStateDesc ->
+                           (LinearScan__IntervalId -> a1) -> (LinearScan__Vec
+                           a1) -> LinearScan__IntervalId -> Vector0.Coq_t 
+                           a1
+_LinearScan__atRegister sd x v i =
+  case _LinearScan__V__nth (_LinearScan__nextInterval sd)
+         (_LinearScan__assignments sd) i of {
+   Prelude.Just r ->
+    Vector0.replace _LinearScan__maxReg (unsafeCoerce v) r (x i);
+   Prelude.Nothing -> unsafeCoerce v}
+
+_LinearScan__registerWithHighestPos :: (Vector1.Vec
+                                       (Prelude.Maybe Prelude.Int)) -> (,)
+                                       Fin0.Coq_fin
+                                       (Prelude.Maybe Prelude.Int)
+_LinearScan__registerWithHighestPos =
+  Vector1.fold_left_with_index _LinearScan__maxReg (\reg res x ->
+    case res of {
+     (,) r o ->
+      case o of {
+       Prelude.Just n ->
+        case x of {
+         Prelude.Just m ->
+          case NPeano.ltb n m of {
+           Prelude.True -> (,) reg (Prelude.Just m);
+           Prelude.False -> (,) r (Prelude.Just n)};
+         Prelude.Nothing -> (,) reg Prelude.Nothing};
+       Prelude.Nothing -> (,) r Prelude.Nothing}}) ((,)
+    (Fin0.from_nat _MyMachine__maxReg 0) (Prelude.Just 0))
+
+_LinearScan__nextIntersectionWith :: Interval.IntervalDesc ->
+                                     LinearScan__ScanStateDesc ->
+                                     LinearScan__IntervalId -> Prelude.Maybe
+                                     Prelude.Int
+_LinearScan__nextIntersectionWith d sd jid =
+  Interval.firstIntersectionPoint
+    (
+      (_LinearScan__V__nth (_LinearScan__nextInterval sd)
+        (_LinearScan__intervals sd) jid)) d
+
 _LinearScan__tryAllocateFreeReg :: LinearScan__ScanStateDesc -> Prelude.Maybe
                                    LinearScan__NextState
 _LinearScan__tryAllocateFreeReg sd =
+  let {freeUntilPos'' = Vector0.const Prelude.Nothing _LinearScan__maxReg} in
   let {
-   freeUntilPos' = _LinearScan__getRegisterIndex sd (\x -> Prelude.Just 0)
-                     (\x -> Prelude.Nothing) (_LinearScan__active sd)}
+   freeUntilPos' = (\f -> Prelude.flip (Data.List.foldl' f))
+                     (unsafeCoerce
+                       (_LinearScan__atRegister sd (\x -> Prelude.Just 0)))
+                     (_LinearScan__active sd) freeUntilPos''}
   in
   let {
    intersectingIntervals = (Prelude.filter) (\x ->
                              Interval.anyRangeIntersects
                                ( (_LinearScan__curIntDetails sd))
-                               ( (_LinearScan__getInterval sd x)))
+                               (
+                                 (_LinearScan__V__nth
+                                   (_LinearScan__nextInterval sd)
+                                   (_LinearScan__intervals sd) x)))
                              (_LinearScan__inactive sd)}
   in
   let {
-   freeUntilPos = _LinearScan__getRegisterIndex sd
-                    (_LinearScan__nextIntersectionWith
-                      ( (_LinearScan__curIntDetails sd)) sd) freeUntilPos'
-                    intersectingIntervals}
+   freeUntilPos = (\f -> Prelude.flip (Data.List.foldl' f))
+                    (unsafeCoerce
+                      (_LinearScan__atRegister sd
+                        (_LinearScan__nextIntersectionWith
+                          ( (_LinearScan__curIntDetails sd)) sd)))
+                    intersectingIntervals freeUntilPos'}
   in
-  let {lastReg = Fin0.ultimate_from_nat _LinearScan__maxReg} in
-  case _LinearScan__findRegister freeUntilPos lastReg of {
+  case _LinearScan__registerWithHighestPos (unsafeCoerce freeUntilPos) of {
    (,) reg mres ->
     let {default0 = _LinearScan__moveUnhandledToActive sd reg} in
     case mres of {
@@ -727,14 +806,19 @@ _LinearScan__checkActiveIntervals sd pos =
        let {
         st1 = case NPeano.ltb
                      (Interval.intervalEnd
-                       ( (_LinearScan__getInterval sd0 ( x)))) pos0 of {
+                       (
+                         (_LinearScan__V__nth (_LinearScan__nextInterval sd0)
+                           (_LinearScan__intervals sd0) ( x)))) pos0 of {
                Prelude.True ->
                 Lib.uncurry_sig (\x0 _ ->
                   _LinearScan__moveActiveToHandled sd0 x0) x;
                Prelude.False ->
                 case (Prelude.not)
                        (Interval.intervalCoversPos
-                         ( (_LinearScan__getInterval sd0 ( x))) pos0) of {
+                         (
+                           (_LinearScan__V__nth
+                             (_LinearScan__nextInterval sd0)
+                             (_LinearScan__intervals sd0) ( x))) pos0) of {
                  Prelude.True ->
                   Lib.uncurry_sig (\x0 _ ->
                     _LinearScan__moveActiveToInactive sd0 x0) x;
@@ -755,13 +839,17 @@ _LinearScan__checkInactiveIntervals sd pos =
        let {
         st1 = case NPeano.ltb
                      (Interval.intervalEnd
-                       ( (_LinearScan__getInterval sd0 ( x)))) pos0 of {
+                       (
+                         (_LinearScan__V__nth (_LinearScan__nextInterval sd0)
+                           (_LinearScan__intervals sd0) ( x)))) pos0 of {
                Prelude.True ->
                 Lib.uncurry_sig (\x0 _ ->
                   _LinearScan__moveInactiveToHandled sd0 x0) x;
                Prelude.False ->
                 case Interval.intervalCoversPos
-                       ( (_LinearScan__getInterval sd0 ( x))) pos0 of {
+                       (
+                         (_LinearScan__V__nth (_LinearScan__nextInterval sd0)
+                           (_LinearScan__intervals sd0) ( x))) pos0 of {
                  Prelude.True ->
                   Lib.uncurry_sig (\x0 _ ->
                     _LinearScan__moveInactiveToActive sd0 x0) x;
