Data/Peano.hs
@@ -3,15 +3,6 @@ module Data.Peano where
 import qualified Prelude
 import qualified Data.List
 
-pred :: Prelude.Int -> Prelude.Int
-pred n =
-  (\fO fS n -> if n Prelude.== 0 then fO () else fS (n Prelude.- 1))
-    (\_ ->
-    n)
-    (\u ->
-    u)
-    n
-
 minus :: Prelude.Int -> Prelude.Int -> Prelude.Int
 minus n m =
   (\fO fS n -> if n Prelude.== 0 then fO () else fS (n Prelude.- 1))
