Data/Vector0.hs
@@ -1,0 +1,37 @@
+module Data.Vector0 where
+
+import qualified Prelude
+import qualified Data.List
+import qualified Data.Fin as Fin
+
+
+__ :: any
+__ = Prelude.error "Logical or arity value used"
+
+data Coq_t a =
+   Coq_nil
+ | Coq_cons a Prelude.Int (Coq_t a)
+
+caseS :: (a1 -> Prelude.Int -> (Coq_t a1) -> a2) -> Prelude.Int -> (Coq_t 
+         a1) -> a2
+caseS h n v =
+  case v of {
+   Coq_nil -> __;
+   Coq_cons h0 n0 t -> h h0 n0 t}
+
+const :: a1 -> Prelude.Int -> Coq_t a1
+const a n =
+  (\fO fS n -> if n Prelude.== 0 then fO () else fS (n Prelude.- 1))
+    (\_ ->
+    Coq_nil)
+    (\n0 -> Coq_cons a n0
+    (const a n0))
+    n
+
+replace :: Prelude.Int -> (Coq_t a1) -> Fin.Coq_t -> a1 -> Coq_t a1
+replace n v p a =
+  case p of {
+   Fin.F1 k -> caseS (\h n0 t -> Coq_cons a n0 t) k v;
+   Fin.FS k p' ->
+    caseS (\h n0 t p2 -> Coq_cons h n0 (replace n0 t p2 a)) k v p'}
+
