LinearScan.hs
@@ -6,7 +6,6 @@ module LinearScan
     , IntervalId
     , handledIntervalIds
     , Interval
-    , getInterval
     , PhysReg
     , registerAssignment
     ) where
@@ -15,7 +14,6 @@ import           Control.Applicative
 import           Data.Fin0
 import qualified Data.Interval as I
 import           Data.Main
-import           Data.Specif
 
 type    VirtReg    = Int
 newtype Graph a    = Graph (LinearScan__Graph a)
@@ -34,10 +32,12 @@ handledIntervalIds :: ScanState -> [IntervalId]
 handledIntervalIds (ScanState (LinearScan__Build_ScanStateDesc ni _ _ _ hnd _ _ _)) =
     map (fin_to_nat ni) hnd
 
-getInterval :: ScanState -> IntervalId -> Interval
-getInterval (ScanState (LinearScan__Build_ScanStateDesc ni _ _ _ _ f _ _)) n =
-    Interval (f (from_nat ni n))
+-- getInterval :: ScanState -> IntervalId -> Interval
+-- getInterval (ScanState (LinearScan__Build_ScanStateDesc ni _ _ _ _ f _ _)) n =
+--     Interval (f (from_nat ni n))
 
 registerAssignment :: ScanState -> IntervalId -> Maybe PhysReg
 registerAssignment (ScanState (LinearScan__Build_ScanStateDesc ni _ _ _ _ _ f _)) n =
-    PhysReg <$> f (from_nat ni n)
+    -- jww (2014-10-01): Allow the Haskell caller to specific the maximum
+    -- number of registers.
+    PhysReg <$> _LinearScan__V__nth _LinearScan__maxReg f (from_nat ni n)
