Vector.v
@@ -1,0 +1,30 @@
+Require Import Fin.
+
+Require Import Coq.Arith.Compare_dec.
+Require Import Coq.Arith.Lt.
+Require Import Coq.Classes.RelationClasses.
+Require Import Coq.Init.Logic.
+Require Import Coq.Numbers.Natural.Peano.NPeano.
+Require Coq.Vectors.Vector.
+
+Open Scope nat_scope.
+
+Module V := Coq.Vectors.Vector.
+Definition Vec := V.t.
+
+Module Import VN := Vector.VectorNotations.
+Module Import EQ := EqNotations.
+
+Definition relocate {A n} (v : Vec A n) (p q : fin n) : Vec A n :=
+  V.replace v q (V.nth v p).
+
+Definition fold_left_with_index {A B : Type} {n} (f : fin n -> B -> A -> B)
+  : forall (b : B) (v : Vec A n), B.
+  intros b v.
+  induction v.
+    apply b.
+  apply IHv.
+  intros.
+  apply fin_expand in H.
+  apply (f H X X0).
+Defined.
